finish context lookup

Capybara/Syntax/Context.lean
@@ -1,5 +1,45 @@
+import Mathlib.Data.Fin.Basic
 import Capybara.Syntax.Type
 namespace Capybara
+
+/-!
+Type binding and capture set binding.
+
+Type binding can be either a type parameter (abstract) or
+a concrete type alias. Similarly, capture set binding can be
+a capture set parameter (abstract) or a concrete capture set alias.
+-/
+inductive TBinding : Nat -> Nat -> Nat -> Type where
+| param : SType n m k -> TBinding n m k
+| alias : SType n m k -> TBinding n m k
+
+inductive CBinding : Nat -> Nat -> Type where
+| param : Kind -> CBinding n k
+| alias : CaptureSet n k -> CBinding n k
+
+notation:max "tparam" S => TBinding.param S
+notation:max "talias" S => TBinding.alias S
+notation:max "cparam" k => CBinding.param k
+notation:max "calias" C => CBinding.alias C
+
+/-!
+Weakening functions for type and capture set binding.
+-/
+def TBinding.weaken : TBinding n m k -> TBinding (n+1) m k
+| TBinding.param T => TBinding.param (T.weaken)
+| TBinding.alias T => TBinding.alias (T.weaken)
+def CBinding.weaken : CBinding n k -> CBinding (n+1) k
+| CBinding.param k => CBinding.param k
+| CBinding.alias C => CBinding.alias (C.weaken)
+def TBinding.tweaken : TBinding n m k -> TBinding n (m+1) k
+| TBinding.param T => TBinding.param (T.tweaken)
+| TBinding.alias T => TBinding.alias (T.tweaken)
+def TBinding.cweaken : TBinding n m k -> TBinding n m (k+1)
+| TBinding.param T => TBinding.param (T.cweaken)
+| TBinding.alias T => TBinding.alias (T.cweaken)
+def CBinding.cweaken : CBinding n k -> CBinding n (k+1)
+| CBinding.param k => CBinding.param k
+| CBinding.alias C => CBinding.alias (C.cweaken)
 
 /-!
 An indexed context. A `Context n m k` contains `n` term variables,
@@ -8,7 +48,57 @@ An indexed context. A `Context n m k` contains `n` term variables,
 inductive Context : Nat -> Nat -> Nat -> Type where
 | empty : Context 0 0 0
 | cons : Context n m k -> CType n m k -> Context (n+1) m k
-| tcons : Context n m k -> SType n m k -> Context n (m+1) k
-| ccons : Context n m k -> CaptureSet n k -> Context n m (k+1)
+| tcons : Context n m k -> TBinding n m k -> Context n (m+1) k
+| ccons : Context n m k -> CBinding n k -> Context n m (k+1)
+
+instance : EmptyCollection (Context 0 0 0) :=
+  ⟨Context.empty⟩
+
+theorem Context.empty_def :
+  ({} : Context 0 0 0) = Context.empty := rfl
+
+notation:20 Γ ",x:" T => Context.cons Γ T
+notation:20 Γ ",X:" T => Context.tcons Γ T
+notation:20 Γ ",c:" C => Context.ccons Γ C
+
+/-!
+Context lookup.
+
+`Context.Lookup`, `Context.LookupT`, and `Context.LookupC` look up the three dimensions of a context,
+respectively.
+-/
+inductive Context.Lookup : Context n m k -> Fin n -> CType n m k -> Prop where
+| here : Context.Lookup (Γ,x:T) 0 T.weaken
+| there :
+  Context.Lookup Γ x T ->
+  Context.Lookup (Γ,x:T) (x.succ) T.weaken
+| tthere :
+  Context.Lookup Γ x T ->
+  Context.Lookup (Γ,X:B) x (T.tweaken)
+| cthere :
+  Context.Lookup Γ x T ->
+  Context.Lookup (Γ,c:B) x (T.cweaken)
+inductive Context.LookupT : Context n m k -> Fin m -> TBinding n m k -> Prop where
+| here : Context.LookupT (Γ,X:T) 0 T.tweaken
+| there :
+  Context.LookupT Γ X S ->
+  Context.LookupT (Γ,x:T) X S.weaken
+| tthere :
+  Context.LookupT Γ X T ->
+  Context.LookupT (Γ,X:B) (X.succ) T.tweaken
+| cthere :
+  Context.LookupT Γ X T ->
+  Context.LookupT (Γ,c:B) X T.cweaken
+inductive Context.LookupC : Context n m k -> Fin k -> CBinding n k -> Prop where
+| here : Context.LookupC (Γ,c:C) 0 C.cweaken
+| there :
+  Context.LookupC Γ c C ->
+  Context.LookupC (Γ,x:T) c C.weaken
+| tthere :
+  Context.LookupC Γ c C ->
+  Context.LookupC (Γ,X:B) c C
+| cthere :
+  Context.LookupC Γ c C ->
+  Context.LookupC (Γ,c:B) (c.succ) C.cweaken
 
 end Capybara
